Lsc3.lean
@@ -17,6 +17,7 @@ import Lsc3.Compile.GetContract
 import Lsc3.Compile.GetMiss
 import Lsc3.Compile.IncBody
 import Lsc3.Compile.IncByBody
+import Lsc3.Compile.IncByHit
 import Lsc3.Compile.IncOverflow
 import Lsc3.Compile.GetInc
 import Lsc3.Compile.GetIncHit
